theories/region_invariants_allocation.v
@@ -138,6 +138,28 @@ Section region_alloc.
       rewrite lookup_insert_ne;auto. iSplitR;[auto|]. iFrame.
   Qed.
 
+  Lemma extend_region_temp E W C a v p φ `{∀ Wv, Persistent (φ Wv)}:
+    isO p = false ->
+    a ∉ dom (std W) →
+    (if isWL p then future_pub_mono C φ v else
+       (if isDL p then future_borrow_mono C φ v else future_priv_mono C φ v)) -∗
+    sts_full_world W C -∗
+    region W C -∗
+    a ↦ₐ v -∗
+    φ (W,C,v)
+
+    ={E}=∗
+
+    region (<s[a := Temporary ]s>W) C
+    ∗ rel C a p φ
+    ∗ sts_full_world (<s[a := Temporary ]s>W) C.
+  Proof.
+    iIntros (HnpO Hnone1) "#HmonoV Hfull Hreg Hl #Hφ".
+    destruct (isWL p) eqn:Hpwl.
+    + iApply (extend_region_temp_pwl with "[$] [$] [$] [$]"); eauto.
+    + iApply (extend_region_temp_nwl with "[$] [$] [$] [$]"); eauto.
+  Qed.
+
   Lemma extend_region_perm E W C a v p φ `{∀ Wv, Persistent (φ Wv)}:
     isO p = false ->
      a ∉ dom (std W) →
@@ -292,6 +314,63 @@ Section region_alloc.
         rewrite /std in H0.
         by iFrame "#∗".
   Qed.
+
+  Lemma extend_region_temp_sepL2 E W C l1 l2 p φ `{∀ Wv, Persistent (φ Wv)}:
+    isO p = false ->
+    Forall (λ k, std W !! k = None) l1 →
+    sts_full_world W C
+    -∗ region W C
+    -∗ ([∗ list] k;v ∈ l1;l2,
+          k ↦ₐ v
+          ∗ φ (W, C, v)
+          ∗ (if isWL p then future_pub_mono C φ v else
+               (if isDL p then future_borrow_mono C φ v else future_priv_mono C φ v)) )
+
+    ={E}=∗
+
+    region (std_update_multiple W l1 Temporary) C
+    ∗ ([∗ list] k ∈ l1, rel C k p φ)
+    ∗ sts_full_world (std_update_multiple W l1 Temporary) C.
+  Proof.
+    revert l2. induction l1.
+    - cbn. intros. iIntros "? ?". iFrame. eauto.
+    - intros l2 HneqO [HWa Hnone_l1]%Forall_cons_1. iIntros "Hsts Hr Hl".
+      simpl.
+      iDestruct (big_sepL2_length with "Hl") as %Hlen.
+      iDestruct (NoDup_of_sepL2_exclusive with "[] Hl") as %[Hal1 ND]%NoDup_cons.
+      { iIntros (? ? ?) "(H1 & ? & ?) (H2 & ? & ?)".
+        iApply (addr_dupl_false with "H1 H2"). }
+      destruct l2; [ by inversion Hlen |].
+      iDestruct (big_sepL2_cons with "Hl") as "[(Ha & Hφ & #Hf) Hl]".
+
+      iMod (IHl1 with "Hsts Hr Hl") as "(Hr & ? & Hsts)"; auto.
+      iDestruct (extend_region_temp with "Hf Hsts Hr Ha [Hφ]") as ">(? & ? & ?)"; eauto.
+      {
+        intro Hcontra.
+        apply elem_of_dom_std_multiple_update in Hcontra.
+        destruct Hcontra as [?|Hcontra]; first set_solver.
+        rewrite elem_of_dom in Hcontra.
+        destruct Hcontra as [? Hcontra].
+        by rewrite Hcontra in HWa.
+      }
+      { destruct (isWL p).
+        + iApply ("Hf" with "[] Hφ"). iPureIntro.
+          apply related_sts_pub_update_multiple.
+          eapply Forall_impl; eauto.
+          intros. by rewrite not_elem_of_dom.
+        + destruct (isDL p).
+          ++ iApply ("Hf" with "[] Hφ"). iPureIntro.
+             apply related_sts_pub_borrow_world, related_sts_pub_update_multiple.
+             eapply Forall_impl; eauto.
+             intros. by rewrite not_elem_of_dom.
+          ++ iApply ("Hf" with "[] Hφ"). iPureIntro.
+             apply related_sts_pub_priv_world, related_sts_pub_update_multiple.
+             eapply Forall_impl; eauto.
+             intros. by rewrite not_elem_of_dom.
+      }
+      iModIntro. cbn. iFrame.
+  Qed.
+
 
   Lemma extend_region_perm_sepL2 E W C l1 l2 p φ `{∀ Wv, Persistent (φ Wv)}:
     isO p = false ->
